x86/PadNopsproof.v
@@ -1,0 +1,55 @@
+(* *******************  *)
+(* Author: Yuting Wang  *)
+(* Date:   Dec 2, 2019 *)
+(* *******************  *)
+
+Require Import Coqlib Errors.
+Require Import Integers Floats AST Linking.
+Require Import Values Memory Events Globalenvs Smallstep.
+Require Import Op Locations Mach Conventions Asm RealAsm.
+Require Import PadNops.
+Import ListNotations.
+Require AsmFacts.
+
+Definition match_prog (p tp:Asm.program) :=
+  match_program (fun _ f tf => tf = transf_fundef f) eq p tp.
+
+Lemma transf_program_match:
+  forall p tp, transf_program p = tp -> match_prog p tp.
+Proof.
+  intros. subst. red. 
+  eapply match_transform_program; eauto.
+Qed.
+
+
+Section PRESERVATION.
+  Existing Instance inject_perm_all.
+Context `{external_calls_prf: ExternalCalls}.
+
+Local Existing Instance mem_accessors_default.
+
+
+Variable prog: Asm.program.
+Variable tprog: Asm.program.
+
+Let ge := Genv.globalenv prog.
+Let tge := Genv.globalenv tprog.
+
+Hypothesis TRANSF: match_prog prog tprog.
+
+Lemma transf_program_correct:
+  forall rs, forward_simulation (semantics prog rs) (semantics tprog rs).
+Proof.
+Admitted.
+
+Lemma transl_fun_pres_stacksize: forall f tf,
+    transl_function f = tf -> 
+    Asm.fn_stacksize f = Asm.fn_stacksize tf.
+Proof.
+  intros f tf HFunc.
+  unfold transl_function in HFunc.
+  subst.
+  simpl. auto.
+Qed.
+
+End PRESERVATION.
